more results about sccs and defined and implemented transpose for graphs

AdjacencyMap.v
@@ -15,17 +15,22 @@ Module AdjacencyMap(O: UsualOrderedType)(S: FSetInterface.Sfun O)(M: FMapInterfa
 
   (*We represent graphs as a map from vertices to sets of edges (neighbors). However, we want to make sure that
     the map is well-formed (mainly this means that if an edge exists in the graph, then both endpoints must
-    exist. So we define a wf predicate and instantiate the graph as a dependent type*)
+    exist.) So we define a wf predicate and instantiate the graph as a dependent type.
+    Additionally, to implement transpose efficiently (in constant time) we store both incoming and outgoing edges.
+    This makes add edge less efficient (though it is asympotically equal), but makes transpose MUCH faster
+    (O(1) instead of O(nlogn) for a balanced BST map*)
   
-  Definition graph_all := M.t (S.t).
+  (*outgoing edges, incoming edges*)
+  Definition graph_all : Type := (M.t (S.t) *  M.t (S.t)).
   
-  Definition contains_vertex_all (g: graph_all) v := M.mem v g.
+  Definition contains_vertex_all (g: graph_all) v := M.mem v (fst g).
 
-  Definition add_vertex_all (g: graph_all) v := if (contains_vertex_all g v) then g else M.add v (S.empty) g.
+  Definition add_vertex_all (g: graph_all) v := if (contains_vertex_all g v) then g else 
+    (M.add v (S.empty) (fst g), M.add v (S.empty) (snd g)).
 
-  Definition empty_all : graph_all := (M.empty (S.t)).
+  Definition empty_all : graph_all := (M.empty (S.t), M.empty (S.t)).
 
-  Definition add_edge_all (g: graph_all) u v := 
+  Definition add_edge_one (g: M.t (S.t)) u v  : M.t (S.t) :=
     match (M.find u g) with
     | None => g
     | Some s => match (M.find v g) with
@@ -34,10 +39,130 @@ Module AdjacencyMap(O: UsualOrderedType)(S: FSetInterface.Sfun O)(M: FMapInterfa
                 end
     end.
 
+  Definition add_edge_all (g: graph_all) u v :=
+    (add_edge_one (fst g) u v, add_edge_one (snd g) v u).
+
+  Definition contains_edge_one (g: M.t S.t) u v : bool :=
+    match (M.find u g) with
+    | None => false
+    | Some s => S.mem v s
+    end.
+
   Inductive wf_graph : graph_all -> Prop :=
   | emp: wf_graph empty_all
   | addv: forall g v, wf_graph g -> wf_graph (add_vertex_all g v)
   | adde: forall g u v, wf_graph g -> wf_graph (add_edge_all g u v).
+
+  Lemma find_mem_some: forall {A: Type} m x (y: A),
+    M.find x m = Some y ->
+    M.mem x m = true.
+  Proof.
+    intros.  assert (M.find x m <> None). intro. rewrite H0 in H. inversion H.
+    eapply P'.F.in_find_iff in H0. apply P'.F.mem_in_iff. apply H0.
+  Qed.
+
+  Lemma find_mem_none: forall {A: Type} (m: M.t A) x,
+    M.find x m = None <->
+    M.mem x m = false.
+  Proof.
+    intros. setoid_rewrite <- P'.F.not_find_in_iff. apply P'.F.not_mem_in_iff.
+  Qed.
+
+(*Two important lemmas that characterize the two different maps*)
+
+  (*Both maps have the same vertices*)
+  Lemma wf_graph_vertices: forall (g: graph_all) v,
+    wf_graph g ->
+    M.mem v (fst g) = true <-> M.mem v (snd g) = true.
+  Proof.
+    intros. revert v. induction H; intros.
+    - simpl in *. rewrite P'.F.empty_a. reflexivity.
+    - unfold add_vertex_all. destruct (contains_vertex_all g v) eqn : ?.
+      + apply IHwf_graph.
+      + simpl. destruct (O.eq_dec v v0). unfold O.eq in e. subst. rewrite P'.F.add_eq_b.
+        rewrite P'.F.add_eq_b. reflexivity. reflexivity. reflexivity. 
+        rewrite P'.F.add_neq_b. rewrite P'.F.add_neq_b. apply IHwf_graph. auto. auto.
+    - unfold add_edge_all. simpl. unfold add_edge_one in *. destruct (M.find u (fst g)) eqn : ?.
+      apply find_mem_some in Heqo. destruct (M.find v (fst g)) eqn : ?.
+      apply find_mem_some in Heqo0. rewrite IHwf_graph in Heqo0. destruct (M.find v (snd g)) eqn : ?.
+      destruct (M.find u (snd g)) eqn : ?. destruct (O.eq_dec v0 u). unfold O.eq in e. subst.
+      rewrite P'.F.add_eq_b. split; intros. rewrite P'.F.add_b. apply orb_true_iff. right. apply IHwf_graph.
+      apply Heqo. reflexivity. reflexivity. rewrite P'.F.add_neq_b. destruct (O.eq_dec v0 v).
+      unfold O.eq in e. subst. rewrite P'.F.add_eq_b. rewrite IHwf_graph. rewrite Heqo0. reflexivity.
+      reflexivity. rewrite P'.F.add_neq_b. apply IHwf_graph. auto. auto. 
+      apply find_mem_none in Heqo2. apply IHwf_graph in Heqo. rewrite Heqo2 in Heqo. inversion Heqo.
+      apply find_mem_none in Heqo1. rewrite Heqo1 in Heqo0. inversion Heqo0.
+      rewrite find_mem_none in Heqo0.
+      destruct (M.mem v (snd g)) eqn : ?. apply IHwf_graph in Heqb. rewrite Heqb in Heqo0. inversion Heqo0.
+      apply find_mem_none in Heqb. rewrite Heqb. apply IHwf_graph.
+      destruct (M.find u (snd g)) eqn : ?. apply find_mem_some in Heqo0. apply find_mem_none in Heqo.
+      apply IHwf_graph in Heqo0. rewrite Heqo0 in Heqo. inversion Heqo. destruct (M.find v (snd g)); apply IHwf_graph.
+Qed.
+
+(*An edge (u,v) is in the first map iff (v,u) is in the second map (this is why transpose is very efficient)*)
+  Lemma wf_graph_edges: forall g u v,
+    wf_graph g ->
+    contains_edge_one (fst g) u v = true <-> contains_edge_one (snd g) v u = true.
+  Proof.
+    intros. revert u. revert v. induction H; intros; unfold contains_edge_one in *; simpl in *.
+    - rewrite P'.F.empty_o. rewrite P'.F.empty_o. reflexivity.
+    - unfold add_vertex_all. destruct (contains_vertex_all g v) eqn : ?; simpl. apply IHwf_graph.
+      destruct (O.eq_dec u v). unfold O.eq in e. subst.
+      rewrite P'.F.add_eq_o. destruct (O.eq_dec v0 v). unfold O.eq in e. subst.
+      rewrite P'.F.add_eq_o. reflexivity. reflexivity. rewrite P'.F.add_neq_o.
+      rewrite <- IHwf_graph. unfold contains_vertex_all in Heqb. apply find_mem_none in Heqb. rewrite Heqb.
+      rewrite P.Dec.F.empty_b. reflexivity. auto. reflexivity.
+      rewrite P'.F.add_neq_o. unfold contains_vertex_all in Heqb. destruct (O.eq_dec v0 v). unfold O.eq in e.
+      subst. rewrite P'.F.add_eq_o. rewrite IHwf_graph.
+      destruct (M.mem v (snd g)) eqn : ?.
+      apply wf_graph_vertices in Heqb0. rewrite Heqb0 in Heqb. inversion Heqb. apply H.
+      apply find_mem_none in Heqb0. rewrite Heqb0. rewrite P.Dec.F.empty_b. reflexivity. reflexivity.
+      rewrite P'.F.add_neq_o. apply IHwf_graph. auto. auto.
+    - unfold add_edge_one. simpl. destruct (M.find u (fst g)) eqn : ?.
+      + assert (exists t, M.find u (snd g) = Some t). { destruct (M.find u (snd g)) eqn : ?.
+        exists t0. reflexivity. apply find_mem_some in Heqo. apply wf_graph_vertices in Heqo.
+        apply find_mem_none in Heqo0. rewrite Heqo0 in Heqo. inversion Heqo. apply H. }
+        destruct_all. rewrite H0. destruct (M.find v (fst g)) eqn : A.
+        * assert (exists t, M.find v (snd g) = Some t). { destruct (M.find v (snd g)) eqn : ?.
+        exists t1. reflexivity. apply find_mem_some in A. apply wf_graph_vertices in A.
+        apply find_mem_none in Heqo0. rewrite Heqo0 in A. inversion A. apply H. }
+        destruct_all. rewrite H1. destruct (O.eq_dec u0 u). unfold O.eq in e. subst.
+        rewrite P'.F.add_eq_o. destruct (O.eq_dec v v0). unfold O.eq in e. subst.
+        rewrite P'.F.add_eq_o. rewrite P.FM.add_b. rewrite P.FM.add_b.
+        unfold P.FM.eqb. destruct (O.eq_dec v0 v0). destruct (O.eq_dec u u). reflexivity.
+        exfalso. apply n. reflexivity. exfalso. apply n. reflexivity. reflexivity.
+        rewrite P'.F.add_neq_o. rewrite P.FM.add_b. rewrite <- IHwf_graph. rewrite Heqo.
+        unfold P.FM.eqb. destruct (O.eq_dec v v0). contradiction. simpl. reflexivity.
+        auto. reflexivity. rewrite P'.F.add_neq_o. destruct (O.eq_dec v0 v). unfold O.eq in e.
+        subst. rewrite P'.F.add_eq_o. rewrite IHwf_graph. rewrite H1. rewrite P.FM.add_b.
+        unfold P.FM.eqb. destruct (O.eq_dec u u0). intuition. reflexivity. reflexivity.
+        rewrite P'.F.add_neq_o. apply IHwf_graph. auto. auto.
+        * assert (M.find v (snd g) = None). { destruct (M.find v (snd g)) eqn : ?.
+          apply find_mem_some in Heqo0. apply wf_graph_vertices in Heqo0.
+          apply find_mem_none in A. rewrite Heqo0 in A. inversion A. apply H. reflexivity. }
+          rewrite H1. apply IHwf_graph.
+      + assert (M.find u (snd g) = None). { destruct (M.find u (snd g)) eqn : ?.
+          apply find_mem_some in Heqo0. apply wf_graph_vertices in Heqo0.
+          apply find_mem_none in Heqo. rewrite Heqo0 in Heqo. inversion Heqo. apply H. reflexivity. }
+        rewrite H0. destruct (M.find v (snd g)); apply IHwf_graph.
+Qed.
+
+  Definition transpose (g: graph_all) := (snd g, fst g).
+
+  Lemma transpose_wf: forall g,
+    wf_graph g ->
+    wf_graph (transpose g).
+  Proof.
+    intros. unfold transpose. induction H; simpl in *.
+    - constructor.
+    - unfold add_vertex_all. destruct (contains_vertex_all g v) eqn : ?.
+      apply IHwf_graph. simpl. eapply addv in IHwf_graph. unfold add_vertex_all in IHwf_graph.
+      unfold contains_vertex_all in *. simpl in *. 
+      destruct (M.mem v (snd g)) eqn : ?. apply wf_graph_vertices in Heqb0. rewrite Heqb0 in Heqb.
+      inversion Heqb. apply H. rewrite Heqb0 in IHwf_graph. apply IHwf_graph.
+    - unfold add_edge_one. assert (A:= IHwf_graph). eapply adde in A. unfold add_edge_all in A.
+      simpl in *. unfold add_edge_one in A. simpl in *. apply A.
+  Qed.
 
   Definition graph := {g: graph_all | wf_graph g}.
 
@@ -49,38 +174,42 @@ Module AdjacencyMap(O: UsualOrderedType)(S: FSetInterface.Sfun O)(M: FMapInterfa
     contains_vertex_all (proj1_sig g) v.
 
   Definition contains_edge (g: graph) (u v : vertex) : bool :=
-    match (M.find u (proj1_sig g)) with
-    | None => false
-    | Some s => S.mem v s
-    end.
+    contains_edge_one (fst (proj1_sig g)) u v.
 
   Definition add_vertex (g: graph)(v: vertex) : graph.
+  Proof.
     unfold graph. econstructor. apply (addv (proj1_sig g) v). unfold graph in g.
     destruct g. simpl. apply w. 
   Defined.
 
-  Definition add_edge (g: graph)( u v: vertex) : graph. 
+  Definition add_edge (g: graph)( u v: vertex) : graph.
+  Proof. 
     unfold graph in *. econstructor. apply (adde (proj1_sig g) u v). destruct g. simpl. apply w.
   Defined.
 
   Definition neighbors_list (g: graph) (v: vertex) : option (list vertex) :=
-    match (M.find v (proj1_sig g)) with
+    match (M.find v (fst(proj1_sig g))) with
     | None => None
     | Some s => Some (S.elements s)
     end.
 
   Definition neighbors_set (g: graph) (v: vertex) : option (S.t) :=
-    M.find v (proj1_sig g).
+    M.find v (fst(proj1_sig g)).
 
   Definition fst_list {A B} (l : list (A * B)) : list A :=
     fold_right (fun (x : A * B) t => let (a,b) := x in a ::t) nil l.
 
   Definition list_of_graph (g: graph) : list vertex :=
-    fst_list (M.elements (proj1_sig g)).
+    fst_list (M.elements (fst(proj1_sig g))).
 
   (*Couldn't find a better function in the interface, so have to add each element*)
   Definition set_of_graph (g: graph) : S.t :=
     fold_right (fun x t => S.add x t) S.empty (list_of_graph g).
+
+  Definition get_transpose (g:graph) : graph.
+  Proof.
+    unfold graph in *. destruct g. apply transpose_wf in w. econstructor. apply w. 
+  Defined.
 
   (*Theories*)
 
@@ -91,9 +220,11 @@ Module AdjacencyMap(O: UsualOrderedType)(S: FSetInterface.Sfun O)(M: FMapInterfa
          | [ H: _ |- _] => progress (unfold empty in *; simpl)
          | [ H: _ |- _] => progress (unfold add_vertex in *; simpl)
          | [ H: _ |- _] => progress (unfold add_vertex_all in *; simpl)
+         | [ H: _ |- _] => progress (unfold add_edge_one in *; simpl)
          | [ H: _ |- _] => progress (unfold add_edge in *; simpl)
          | [ H: _ |- _] => progress (unfold add_edge_all in *; simpl)
          | [ H: _ |- _] => progress (unfold contains_edge in *; simpl)
+         | [ H: _ |- _] => progress (unfold contains_edge_one in *; simpl)
          | [ H: _ |- _] => progress (unfold empty_all in *; simpl)
          end). 
 
@@ -112,7 +243,7 @@ Module AdjacencyMap(O: UsualOrderedType)(S: FSetInterface.Sfun O)(M: FMapInterfa
   Lemma add_vertex_1: forall g v,
     contains_vertex (add_vertex g v) v = true.
   Proof.
-    intros. unfold_all. destruct g. simpl. destruct (M.mem v x) eqn : ?.
+    intros. unfold_all. destruct g. simpl. destruct (M.mem v (fst x)) eqn : ?.
     - apply Heqb.
     - apply M.mem_1. unfold M.In. exists S.empty. apply M.add_1. reflexivity.
   Qed.
@@ -122,7 +253,7 @@ Module AdjacencyMap(O: UsualOrderedType)(S: FSetInterface.Sfun O)(M: FMapInterfa
     contains_vertex g u = true.
   Proof.
     intros. unfold_all. destruct g; simpl in *. 
-    destruct (M.find u x) eqn : ?.
+    destruct (M.find u (fst x)) eqn : ?.
     - rewrite P'.F.mem_find_b. rewrite Heqo. reflexivity.
     - inversion H.
   Qed.
@@ -131,25 +262,25 @@ Module AdjacencyMap(O: UsualOrderedType)(S: FSetInterface.Sfun O)(M: FMapInterfa
     contains_edge g u v = true ->
     contains_vertex g v = true.
   Proof.
-    intros. unfold_all; destruct g; simpl in *. destruct (M.find u x) eqn : ?. generalize dependent t.
+    intros. unfold_all; destruct g; simpl in *. destruct (M.find u (fst x)) eqn : ?. generalize dependent t.
      induction w; intros; try(unfold_all).
     - rewrite P'.F.empty_o in Heqo. inversion Heqo.
-    - destruct (M.mem v0 g) eqn : ?.
+    - destruct (M.mem v0 (fst g)) eqn : ?.
       + eapply IHw. apply Heqo. apply H.
       + destruct (O.eq_dec u v0).
-        * unfold O.eq in e. subst. rewrite P'.F.add_eq_o in Heqo. inversion Heqo; subst.
+        * unfold O.eq in e. subst. simpl in *. rewrite P'.F.add_eq_o in Heqo. inversion Heqo; subst.
           rewrite P.Dec.F.empty_b in H. inversion H. reflexivity.
-        * rewrite P'.F.add_neq_o in Heqo. rewrite P'.F.add_b. apply orb_true_iff.
+        * simpl in *. rewrite P'.F.add_neq_o in Heqo. rewrite P'.F.add_b. apply orb_true_iff.
           right. eapply IHw. apply Heqo. apply H. auto.
-    - destruct (M.find u0 g) eqn : ?.
-      + destruct (M.find v0 g) eqn : ?. destruct (O.eq_dec u u0). unfold O.eq in e. subst.
+    - destruct (M.find u0 (fst g)) eqn : ?.
+      + destruct (M.find v0 (fst g)) eqn : ?. destruct (O.eq_dec u u0). unfold O.eq in e. subst; simpl in *.
         rewrite P'.F.add_eq_o in Heqo. inversion Heqo; subst. destruct (O.eq_dec v v0). unfold O.eq in e.
         subst. destruct (O.eq_dec v0 u0). unfold O.eq in e. subst. rewrite P'.F.add_b.
         apply orb_true_iff. left. unfold P'.F.eqb. destruct (O.eq_dec u0 u0). reflexivity. exfalso.
         apply n. reflexivity. rewrite P'.F.add_b. apply orb_true_iff. right.
         rewrite P'.F.mem_find_b. rewrite Heqo1. reflexivity.
         rewrite P.Dec.F.add_neq_b in H. rewrite P'.F.add_b. apply orb_true_iff. right. eapply IHw.
-        apply Heqo0. apply H. auto. reflexivity. rewrite P'.F.add_neq_o in Heqo. 
+        apply Heqo0. apply H. auto. reflexivity. simpl in *. rewrite P'.F.add_neq_o in Heqo. 
         rewrite P'.F.add_b. apply orb_true_iff. right. eapply IHw. apply Heqo. apply H. auto.
         eapply IHw. apply Heqo. apply H.
       + eapply IHw. apply Heqo. apply H.
@@ -162,8 +293,8 @@ Module AdjacencyMap(O: UsualOrderedType)(S: FSetInterface.Sfun O)(M: FMapInterfa
     contains_edge (add_edge g u v) u v = true.
   Proof.
     intros. unfold_all. destruct g; simpl in *. rewrite P'.F.mem_find_b in H.
-    rewrite P'.F.mem_find_b in H0. destruct (M.find v x) eqn : ?.
-    destruct (M.find u x) eqn : ?. rewrite P'.F.add_eq_o. rewrite P.FM.add_b.
+    rewrite P'.F.mem_find_b in H0. destruct (M.find v (fst x)) eqn : ?.
+    destruct (M.find u (fst x)) eqn : ?. rewrite P'.F.add_eq_o. rewrite P.FM.add_b.
     apply orb_true_iff. left. unfold P.FM.eqb. destruct (O.eq_dec v v). reflexivity.
     exfalso. apply n. reflexivity. reflexivity. inversion H0. inversion H.
   Qed. 
@@ -174,23 +305,23 @@ Module AdjacencyMap(O: UsualOrderedType)(S: FSetInterface.Sfun O)(M: FMapInterfa
   Proof.
     intros. assert (contains_vertex g a = true) by (eapply contains_edge_1; eassumption).
     assert (contains_vertex g b = true) by (eapply contains_edge_2; eassumption).
-     unfold_all. destruct g; simpl in *. destruct (M.find a x) eqn : ?.
-    - destruct (M.find u x) eqn : ?.
+     unfold_all. destruct g; simpl in *. destruct (M.find a (fst x)) eqn : ?.
+    - destruct (M.find u (fst x)) eqn : ?.
       + destruct (O.eq_dec a u) eqn : ?.
         * unfold O.eq in e. subst. destruct (O.eq_dec v b).
-          -- unfold O.eq in e. subst. rewrite P'.F.mem_find_b in H1. destruct (M.find b x) eqn : ?.
+          -- unfold O.eq in e. subst. rewrite P'.F.mem_find_b in H1. destruct (M.find b (fst x)) eqn : ?.
              ++ rewrite P'.F.add_eq_o. rewrite P.Dec.F.add_b. apply orb_true_iff. left.
                 unfold P.Dec.F.eqb. destruct (O.eq_dec b b). reflexivity. exfalso. apply n. reflexivity.
                 reflexivity.
              ++ inversion H1.
-          -- rewrite Heqo0 in Heqo. inversion Heqo; subst. destruct (M.find v x) eqn : ?.
+          -- rewrite Heqo0 in Heqo. inversion Heqo; subst. destruct (M.find v (fst x)) eqn : ?.
              rewrite P'.F.add_eq_o. rewrite P.FM.add_b. apply orb_true_iff. right. apply H. reflexivity.
-             rewrite P'.F.mem_find_b in H0. destruct (M.find u x) eqn : ?. inversion Heqo0; subst.
+             rewrite P'.F.mem_find_b in H0. destruct (M.find u (fst x)) eqn : ?. inversion Heqo0; subst.
              apply H. inversion H0.
-        * clear Heqs. destruct (M.find v x) eqn : ?. rewrite P'.F.add_neq_o. 
-          rewrite P'.F.mem_find_b in H0. destruct (M.find a x). inversion Heqo; subst. apply H. inversion H0.
-          auto. rewrite P'.F.mem_find_b in H0. destruct (M.find a x). inversion Heqo; subst. apply H. inversion Heqo.
-      +  rewrite P'.F.mem_find_b in H0. destruct (M.find a x). inversion Heqo; subst. apply H. inversion Heqo.
+        * clear Heqs. destruct (M.find v (fst x)) eqn : ?. rewrite P'.F.add_neq_o. 
+          rewrite P'.F.mem_find_b in H0. destruct (M.find a (fst x)). inversion Heqo; subst. apply H. inversion H0.
+          auto. rewrite P'.F.mem_find_b in H0. destruct (M.find a (fst x)). inversion Heqo; subst. apply H. inversion Heqo.
+      +  rewrite P'.F.mem_find_b in H0. destruct (M.find a (fst x)). inversion Heqo; subst. apply H. inversion Heqo.
     - inversion H.
   Qed.
  
@@ -198,8 +329,8 @@ Module AdjacencyMap(O: UsualOrderedType)(S: FSetInterface.Sfun O)(M: FMapInterfa
     u <> a \/ v <> b ->
     (contains_edge g a b = contains_edge (add_edge g u v) a b).
   Proof.
-    intros. unfold_all;destruct g; simpl in *. destruct (M.find u x) eqn : ?.
-    destruct (M.find v x) eqn : ?. destruct H.
+    intros. unfold_all;destruct g; simpl in *. destruct (M.find u (fst x)) eqn : ?.
+    destruct (M.find v (fst x)) eqn : ?. destruct H.
     rewrite P'.F.add_neq_o. reflexivity. apply H. destruct (O.eq_dec u a).
     unfold O.eq in e. subst. rewrite P'.F.add_eq_o. rewrite Heqo. rewrite P.Dec.F.add_neq_b.
     reflexivity. apply H. reflexivity. rewrite P'.F.add_neq_o. reflexivity. auto.
@@ -210,10 +341,10 @@ Module AdjacencyMap(O: UsualOrderedType)(S: FSetInterface.Sfun O)(M: FMapInterfa
     contains_vertex g v = false <-> neighbors_list g v = None.
   Proof.
     intros. unfold_all; destruct g; simpl in *. unfold neighbors_list. simpl in *. split; intros.
-    - destruct (M.find v x) eqn : ?. apply M.find_2 in Heqo.
-      assert (M.In v x). unfold M.In. exists t. assumption.
+    - destruct (M.find v (fst x)) eqn : ?. apply M.find_2 in Heqo.
+      assert (M.In v (fst x)). unfold M.In. exists t. assumption.
       apply M.mem_1 in H0. rewrite H0 in H. inversion H. reflexivity.
-    - destruct (M.find v x) eqn : ?. inversion H. destruct (M.mem v x) eqn : ?.
+    - destruct (M.find v (fst x)) eqn : ?. inversion H. destruct (M.mem v (fst x)) eqn : ?.
       apply M.mem_2 in Heqb. unfold M.In in Heqb. destruct Heqb.
       apply M.find_1 in H0. rewrite H0 in Heqo. inversion Heqo. reflexivity.
 Qed.
@@ -223,7 +354,7 @@ Qed.
     contains_edge g u v = true <-> In v l.
   Proof.
     intros. unfold_all; unfold neighbors_list in *; destruct g; simpl in *. 
-    destruct (M.find u x) eqn : ?.
+    destruct (M.find u (fst x)) eqn : ?.
     - inversion H; subst. split; intros. 
       + apply S.mem_2 in H0. apply S.elements_1 in H0. rewrite <- In_InA_equiv in H0. assumption.
       + apply S.mem_1. apply S.elements_2. rewrite <- In_InA_equiv. assumption.
@@ -234,7 +365,7 @@ Qed.
     neighbors_list g v = Some l ->
     StronglySorted (O.lt) l. 
   Proof.
-    intros. unfold neighbors_list in H; destruct g; simpl in *. destruct (M.find v x).
+    intros. unfold neighbors_list in H; destruct g; simpl in *. destruct (M.find v (fst x)).
     - inversion H; subst. apply Sorted_StronglySorted. unfold Relations_1.Transitive.
       intros. eapply O.lt_trans. apply H0. apply H1. apply S.elements_3.
     - inversion H.
@@ -244,7 +375,7 @@ Qed.
     neighbors_set g v = None <-> neighbors_list g v = None.
   Proof.
     intros. unfold neighbors_set. unfold neighbors_list. destruct g; simpl in *. 
-    destruct (M.find v x).
+    destruct (M.find v (fst x)).
     - split; intros H; inversion H.
     - split; intros; reflexivity. 
   Qed.
@@ -278,13 +409,13 @@ Qed.
     intros. unfold_all. unfold list_of_graph. destruct g; simpl in *. split; intros.
     - apply in_fst_list. apply M.mem_2 in H. unfold M.In in H.
       destruct H. exists x0. apply M.elements_1 in H.
-      unfold M.eq_key_elt in H. induction (M.elements x).
+      unfold M.eq_key_elt in H. induction (M.elements (fst x)).
       + rewrite InA_nil in H. destruct H.
       + simpl. rewrite InA_cons in H. destruct H.
         * destruct H. simpl in *. left. subst. destruct a. simpl. reflexivity.
         * right. apply IHl. apply H.
     - rewrite <- in_fst_list in H. destruct H. 
-      assert (InA (M.eq_key_elt (elt:=S.t)) (v, x0) (M.elements x)). { induction (M.elements x).
+      assert (InA (M.eq_key_elt (elt:=S.t)) (v, x0) (M.elements (fst x))). { induction (M.elements (fst x)).
       - simpl in H. destruct H.
       - simpl in H. destruct H.
         + destruct a. inversion H; subst. apply InA_cons. left. 
@@ -324,6 +455,19 @@ Qed.
         + right. apply IHl. apply H.
         + apply P.FM.add_iff. destruct H. left. apply H. right. apply IHl. apply H. }
         rewrite list_of_graph_1. rewrite H. reflexivity.
+  Qed.
+
+  Lemma tranpose_vertices: forall g v,
+    contains_vertex g v = true <-> contains_vertex (get_transpose g) v = true.
+  Proof.
+    intros. unfold_all. unfold get_transpose. destruct g. simpl in *. apply wf_graph_vertices.
+    apply w.
+  Qed.
+
+  Lemma transpose_edges: forall g u v,
+    contains_edge g u v = true <-> contains_edge (get_transpose g) v u = true.
+  Proof. 
+    intros. unfold_all. unfold get_transpose. destruct g. simpl in *. apply wf_graph_edges. apply w.
   Qed.
 
   Definition topological_sort l g :=
