Graph.v
@@ -26,6 +26,8 @@ Module Type Graph (O: UsualOrderedType)(S: FSetInterface.Sfun O).
 
   Parameter set_of_graph: graph -> S.t.
 
+  Parameter get_transpose: graph -> graph.
+
   Parameter empty_1: forall v,
     contains_vertex empty v = false.
 
@@ -83,6 +85,12 @@ Module Type Graph (O: UsualOrderedType)(S: FSetInterface.Sfun O).
   Parameter set_of_graph_1: forall g v,
     contains_vertex g v = true <-> S.In v (set_of_graph g).
 
+  Parameter tranpose_vertices: forall g v,
+    contains_vertex g v = true <-> contains_vertex (get_transpose g) v = true.
+
+  Parameter transpose_edges: forall g u v,
+    contains_edge g u v = true <-> contains_edge (get_transpose g) v u = true.
+
   (*TODO: see if better way to define in interface*)
   (*A topological ordering is one where there are no edges going backward in the list and every vertex in the 
   graph is in the list*)
@@ -95,125 +103,3 @@ Module Type Graph (O: UsualOrderedType)(S: FSetInterface.Sfun O).
 
 
 End Graph.
-(*
-Module Transpose (O: UsualOrderedType)(S: FSetInterface.Sfun O) (G: Graph O S) <: Graph O S.
-
-  Definition graph := G.graph.
-
-  Definition empty : graph := G.empty.
-
-  Definition vertex := O.t.
-
-  Definition contains_vertex: graph -> vertex -> bool := G.contains_vertex.
-
-  Definition contains_edge (g: graph )( u v : vertex) : bool :=
-    G.contains_edge g v u.
-
-  Definition add_vertex: graph -> vertex -> graph := G.add_vertex.
-
-  Definition add_edge g u v := G.add_edge g v u.
-
-  Definition neighbors_list: graph -> vertex -> option (list vertex) := G.neighbors_list.
-
-  Definition neighbors_set: graph -> vertex -> option (S.t) := G.neighbors_set.
-
-  Definition list_of_graph: graph -> list vertex := G.list_of_graph.
-
-  Definition set_of_graph: graph -> S.t := G.set_of_graph.
-
-  Lemma empty_1: forall v,
-    contains_vertex empty v = false.
-  Proof. intros. unfold contains_vertex. apply G.empty_1. Qed.
-
-  Lemma empty_2: forall u v,
-    contains_edge empty u v = false.
-  Proof. intros. unfold contains_edge. apply G.empty_2. Qed.
-  
-  Lemma add_vertex_1: forall g v,
-    contains_vertex (add_vertex g v) v = true.
-  Proof. intros. unfold contains_vertex. unfold add_vertex. apply G.add_vertex_1. Qed.
-
-  Lemma contains_edge_1: forall g u v,
-    contains_edge g u v = true ->
-    contains_vertex g u = true.
-  Proof. 
-    intros. unfold contains_vertex. unfold contains_edge in H. eapply G.contains_edge_2. apply H.
-  Qed. 
-
-  Lemma contains_edge_2: forall g u v,
-    contains_edge g u v = true ->
-    contains_vertex g v = true.
-  Proof.
-    intros. unfold contains_vertex. unfold contains_edge in H. eapply G.contains_edge_1. apply H.
-  Qed.
-
-  Lemma add_edge_1: forall g u v,
-    contains_vertex g v = true ->
-    contains_vertex g u = true ->
-    contains_edge (add_edge g u v) u v = true.
-  Proof.
-    intros. unfold contains_edge. unfold add_edge. unfold contains_vertex in *. apply G.add_edge_1; assumption.
-  Qed.
-
-  Lemma add_edge_2: forall g u v a b,
-    contains_edge g a b = true ->
-    contains_edge (add_edge g u v) a b = true.
-  Proof.
-    intros. unfold contains_edge in *. unfold add_edge. apply G.add_edge_2. apply H.
-  Qed.
-
-  Lemma add_edge_3: forall g u v a b,
-    u <> a \/ v <> b ->
-    (contains_edge g a b = contains_edge (add_edge g u v) a b).
-  Proof.
-    intros. unfold contains_edge. unfold add_edge. apply G.add_edge_3. destruct H;
-    try(right; assumption); try(left; assumption).
-  Qed.
-
-  Lemma neighbors_list_1: forall g v,
-    contains_vertex g v = false <-> neighbors_list g v = None.
-  Proof.
-    intros. unfold contains_vertex. unfold neighbors_list. apply G.neighbors_list_1.
-  Qed.
-
-  Lemma neighbors_list_2: forall g u v l,
-    neighbors_list g u = Some l ->
-    contains_edge g u v = true <-> In v l.
-  Proof.
-    intros. unfold neighbors_list in H. unfold contains_edge. eapply G.neighbors_list_2.
-
-  Parameter neighbors_list_3: forall g v l,
-    neighbors_list g v = Some l ->
-    StronglySorted (O.lt) l.
-
-  Parameter neighbors_set_1: forall g v,
-    neighbors_set g v = None <-> neighbors_list g v = None.
-
-  Parameter neighbors_set_2: forall g u v s,
-    neighbors_set g u = Some s ->
-    contains_edge g u v = true <-> S.In v s.
-
-  Parameter list_of_graph_1: forall g v,
-    contains_vertex g v = true <-> In v (list_of_graph g).
-
-  Parameter list_of_graph_2: forall g,
-    StronglySorted (O.lt) (list_of_graph g).
-
-  Parameter set_of_graph_1: forall g v,
-    contains_vertex g v = true <-> S.In v (set_of_graph g).
-
-  (*TODO: see if better way to define in interface*)
-  (*A topological ordering is one where there are no edges going backward in the list and every vertex in the 
-  graph is in the list*)
-  Parameter topological_sort: list vertex -> graph ->  Prop.
-
-  Parameter topological_sort_def: forall l g,
-    topological_sort l g <-> 
-  (forall v, contains_vertex g v = true <-> In v l) /\ NoDup l /\
-  (forall l1 l2 l3 u v, l = l1 ++ u :: l2 ++ v :: l3 -> contains_edge g v u = false).
-
-End Transpose.
-*)
-  
-
-  
